AwsCryptographicMaterialProviders/dafny/AwsCryptographyKeyStore/src/CreateKeys.dfy
@@ -237,14 +237,14 @@ module {:options "/functionSyntax:4" } CreateKeys {
     var activeEncryptionContext := Structure.ActiveBranchKeyEncryptionContext(decryptOnlyEncryptionContext);
     var beaconEncryptionContext := Structure.BeaconKeyEncryptionContext(decryptOnlyEncryptionContext);
 
-    assert KMSKeystoreOperations.AttemptKmsOperation?(kmsConfiguration, decryptOnlyEncryptionContext);
+    assert KMSKeystoreOperations.AttemptKmsOperation?(kmsConfiguration, decryptOnlyEncryptionContext[Structure.KMS_FIELD]);
     var wrappedDecryptOnlyBranchKey :- KMSKeystoreOperations.GenerateKey(
       decryptOnlyEncryptionContext,
       kmsConfiguration,
       grantTokens,
       kmsClient
     );
-    assert KMSKeystoreOperations.AttemptKmsOperation?(kmsConfiguration, activeEncryptionContext);
+    assert KMSKeystoreOperations.AttemptKmsOperation?(kmsConfiguration, activeEncryptionContext[Structure.KMS_FIELD]);
     var wrappedActiveBranchKey :- KMSKeystoreOperations.ReEncryptKey(
       wrappedDecryptOnlyBranchKey.CiphertextBlob.value,
       decryptOnlyEncryptionContext,
@@ -253,7 +253,7 @@ module {:options "/functionSyntax:4" } CreateKeys {
       grantTokens,
       kmsClient
     );
-    assert KMSKeystoreOperations.AttemptKmsOperation?(kmsConfiguration, beaconEncryptionContext);
+    assert KMSKeystoreOperations.AttemptKmsOperation?(kmsConfiguration, beaconEncryptionContext[Structure.KMS_FIELD]);
     var wrappedBeaconKey :- KMSKeystoreOperations.GenerateKey(
       beaconEncryptionContext,
       kmsConfiguration,
@@ -342,7 +342,7 @@ module {:options "/functionSyntax:4" } CreateKeys {
               //# The `KmsArn` of the [EncryptedHierarchicalKey](./key-store/key-storage.md#encryptedhierarchicalkey)
               //# MUST be [compatible with](#aws-key-arn-compatibility)
               //# the configured `KMS ARN` in the [AWS KMS Configuration](#aws-kms-configuration) for this keystore.
-              && KMSKeystoreOperations.AttemptKmsOperation?(kmsConfiguration, oldActiveItem.EncryptionContext)
+              && KMSKeystoreOperations.AttemptKmsOperation?(kmsConfiguration, oldActiveItem.EncryptionContext[Structure.KMS_FIELD])
               && KMSKeystoreOperations.Compatible?(kmsConfiguration, oldActiveItem.KmsArn)
 
               //= aws-encryption-sdk-specification/framework/branch-key-store.md#versionkey
@@ -502,7 +502,7 @@ module {:options "/functionSyntax:4" } CreateKeys {
         message := "At this time, VersionKey ONLY supports HV-1; BK's Active Item is HV-2.")
     );
     :- Need(
-      && KMSKeystoreOperations.AttemptKmsOperation?(kmsConfiguration, oldActiveItem.EncryptionContext),
+      && KMSKeystoreOperations.AttemptKmsOperation?(kmsConfiguration, oldActiveItem.EncryptionContext[Structure.KMS_FIELD]),
       Types.KeyStoreException(
         message := ErrorMessages.VERSION_KEY_KMS_KEY_ARN_DISAGREEMENT)
     );
@@ -524,7 +524,7 @@ module {:options "/functionSyntax:4" } CreateKeys {
 
     var activeEncryptionContext := Structure.ActiveBranchKeyEncryptionContext(decryptOnlyEncryptionContext);
 
-    assert KMSKeystoreOperations.AttemptKmsOperation?(kmsConfiguration, decryptOnlyEncryptionContext);
+    assert KMSKeystoreOperations.AttemptKmsOperation?(kmsConfiguration, decryptOnlyEncryptionContext[Structure.KMS_FIELD]);
 
     var wrappedDecryptOnlyBranchKey :- KMSKeystoreOperations.GenerateKey(
       decryptOnlyEncryptionContext,
